Define head and tail reachability, and show they imply the right types
Following AuxList chains up to but not including the given "last"
pointer, and picking up pointers to head elements or tail AuxLists.

In a wfstate, a non-null pointer reachable by tailR from an AuxList_type
emb.type head will have AuxList_type emb.type, and one reachable by
headR will have emb.type.

hol/ptypesScript.sml
@@ -525,6 +525,90 @@ pop_assum mp_tac >>
  |> match_mp_tac) >>
 srw_tac [][RINTER]);
 
+val tailR1_def = Define`
+  tailR1 s l n1 n2 = n2 ≠ ptr_to_num l ∧ ∃h. FLOOKUP s n2 = SOME (AuxList_value h n1)`;
+val _ = overload_on("tailR", ``λs last. RTC (tailR1 s last)``);
+
+val list_of_AuxList_tailR_type = Q.store_thm(
+"list_of_AuxList_tailR_type",
+`∀p ls. list_of_AuxList emb s l p ls ⇒
+        wfstate s ∧ (s.cell_type (ptr_to_num p) = AuxList_type emb.type) ∧
+        tailR s.store l m (ptr_to_num p) ∧ m ≠ 0 ⇒
+        (s.cell_type m = AuxList_type emb.type)`,
+ho_match_mp_tac list_of_AuxList_ind >>
+conj_tac >- srw_tac [][Once RTC_CASES2,tailR1_def] >>
+srw_tac [][UNCURRY] >>
+fsrw_tac [][] >> srw_tac [][] >>
+qpat_assum `tailR ss l m pp` mp_tac >>
+srw_tac [][Once RTC_CASES2,tailR1_def] >- srw_tac [][] >>
+fsrw_tac [][lookup_succeeds] >>
+qpat_assum `X = FST x` (assume_tac o SYM) >>
+fsrw_tac [][] >>
+`typed_cell s {} (ptr_to_num p)` by
+  fsrw_tac [][FLOOKUP_DEF,wfstate_def,typed_state_def] >>
+pop_assum mp_tac >> asm_simp_tac (srw_ss()) [typed_cell_def] >>
+qmatch_assum_rename_tac `FLOOKUP (SND x).store h = SOME v` [] >>
+Cases_on `x` >> fsrw_tac [][] >>
+srw_tac [][Once has_type_cases] >>
+qpat_assum `tailR ss l m u` mp_tac >>
+srw_tac [][Once RTC_CASES2,tailR1_def] >-
+  (first_x_assum match_mp_tac >> first_assum ACCEPT_TAC) >>
+fsrw_tac [][wfstate_def,FLOOKUP_DEF] >>
+first_x_assum match_mp_tac >>
+first_x_assum match_mp_tac >>
+PROVE_TAC []);
+
+val headR_def = Define`
+  headR s l n1 n2 = ∃a t. tailR s l a n2 ∧ (FLOOKUP s a = SOME (AuxList_value n1 t))`;
+
+val list_of_AuxList_headR_type = Q.store_thm(
+"list_of_AuxList_headR_type",
+`∀p ls. list_of_AuxList emb s l p ls ⇒
+        wfstate s ∧ (s.cell_type (ptr_to_num p) = AuxList_type emb.type) ∧
+        headR s.store l m (ptr_to_num p) ∧ m ≠ 0 ⇒
+        (s.cell_type m = emb.type)`,
+ho_match_mp_tac list_of_AuxList_ind >>
+conj_tac >- (
+  srw_tac [][Once RTC_CASES2,headR_def,tailR1_def] >>
+  fsrw_tac [][FLOOKUP_DEF,wfstate_def,typed_state_def,typed_cell_def] >>
+  res_tac >> pop_assum mp_tac >>
+  simp_tac (srw_ss()) [Once has_type_cases] >>
+  srw_tac [][] ) >>
+srw_tac [][UNCURRY] >>
+fsrw_tac [][] >> srw_tac [][] >>
+qpat_assum `headR ss l m pp` mp_tac >>
+srw_tac [][headR_def,Once RTC_CASES2,tailR1_def] >- (
+  fsrw_tac [][lookup_succeeds,FLOOKUP_DEF,wfstate_def,typed_state_def,typed_cell_def] >>
+  res_tac >> pop_assum mp_tac >>
+  simp_tac (srw_ss()) [Once has_type_cases] >>
+  srw_tac [][] ) >>
+fsrw_tac [][lookup_succeeds] >>
+qpat_assum `X = FST x` (assume_tac o SYM) >>
+fsrw_tac [][] >>
+`typed_cell s {} (ptr_to_num p)` by
+  fsrw_tac [][FLOOKUP_DEF,wfstate_def,typed_state_def] >>
+pop_assum mp_tac >> asm_simp_tac (srw_ss()) [typed_cell_def] >>
+qmatch_assum_rename_tac `FLOOKUP (SND x).store h = SOME v` [] >>
+Cases_on `x` >> fsrw_tac [][] >>
+srw_tac [][Once has_type_cases] >>
+qpat_assum `tailR ss l a u` mp_tac >>
+srw_tac [][Once RTC_CASES2,tailR1_def] >- (
+  first_x_assum match_mp_tac >>
+  fsrw_tac [][FLOOKUP_DEF,wfstate_def] >>
+  `a ≠ 0` by PROVE_TAC [] >>
+  fsrw_tac [][] >>
+  srw_tac [][headR_def,FLOOKUP_DEF] >>
+  srw_tac [][Once RTC_CASES2,tailR1_def,FLOOKUP_DEF] >>
+  PROVE_TAC [] ) >>
+fsrw_tac [][wfstate_def,FLOOKUP_DEF] >>
+first_x_assum match_mp_tac >>
+conj_tac >- (
+  first_x_assum match_mp_tac >>
+  PROVE_TAC [] ) >>
+srw_tac [][headR_def,FLOOKUP_DEF] >>
+srw_tac [][Once RTC_CASES2,tailR1_def,FLOOKUP_DEF] >>
+PROVE_TAC [] );
+
 val AddToFrontOfList_CONS = Q.store_thm(
 "AddToFrontOfList_CONS",
 `is_embed emb ∧ typed_state s0 ∧
